BoogieLang/VCExprHelper.thy
@@ -2,92 +2,94 @@ theory VCExprHelper
 imports Semantics Util
 begin
 
-lemma vc_to_expr:"\<lbrakk>vc; A,\<Gamma> \<turnstile> \<langle>e,ns\<rangle> \<Down> LitV (LBool vc)\<rbrakk> \<Longrightarrow> A,\<Gamma> \<turnstile> \<langle>e,ns\<rangle> \<Down> LitV (LBool True)"
+lemma vc_to_expr:"\<lbrakk>vc; A,\<Gamma>,\<Omega> \<turnstile> \<langle>e,ns\<rangle> \<Down> LitV (LBool vc)\<rbrakk> \<Longrightarrow> A,\<Gamma>,\<Omega> \<turnstile> \<langle>e,ns\<rangle> \<Down> LitV (LBool True)"
   by simp
 
-lemma expr_to_vc:"\<lbrakk>A,\<Gamma> \<turnstile> \<langle>e, ns\<rangle> \<Down> LitV (LBool True); A,\<Gamma> \<turnstile> \<langle>e, ns\<rangle> \<Down> LitV (LBool vc)\<rbrakk> \<Longrightarrow> vc"
+lemma expr_to_vc:"\<lbrakk>A,\<Gamma>,\<Omega> \<turnstile> \<langle>e, ns\<rangle> \<Down> LitV (LBool True); A,\<Gamma>,\<Omega> \<turnstile> \<langle>e, ns\<rangle> \<Down> LitV (LBool vc)\<rbrakk> \<Longrightarrow> vc"
   by (blast dest: expr_eval_determ)
 
 (* boolean operations *)
 lemma conj_vc_rel: 
-  assumes "A,\<Gamma> \<turnstile> \<langle>e1, ns\<rangle> \<Down> LitV (LBool vc1)" and "A,\<Gamma> \<turnstile> \<langle>e2, ns\<rangle> \<Down> LitV (LBool vc2)"
-  shows "A,\<Gamma> \<turnstile> \<langle>e1 \<guillemotleft>And\<guillemotright> e2, ns\<rangle> \<Down> LitV (LBool (vc1 \<and> vc2))"
+  assumes "A,\<Gamma>,\<Omega> \<turnstile> \<langle>e1, ns\<rangle> \<Down> LitV (LBool vc1)" and "A,\<Gamma>,\<Omega> \<turnstile> \<langle>e2, ns\<rangle> \<Down> LitV (LBool vc2)"
+  shows "A,\<Gamma>,\<Omega> \<turnstile> \<langle>e1 \<guillemotleft>And\<guillemotright> e2, ns\<rangle> \<Down> LitV (LBool (vc1 \<and> vc2))"
   using assms
   by (auto intro: RedBinOp)
 
 lemma disj_vc_rel: 
-  assumes "A,\<Gamma> \<turnstile> \<langle>e1, ns\<rangle> \<Down> LitV (LBool vc1)" and "A,\<Gamma> \<turnstile> \<langle>e2, ns\<rangle> \<Down> LitV (LBool vc2)"
-  shows "A,\<Gamma> \<turnstile> \<langle>e1 \<guillemotleft>Or\<guillemotright> e2, ns\<rangle> \<Down> LitV (LBool (vc1 \<or> vc2))"
+  assumes "A,\<Gamma>,\<Omega> \<turnstile> \<langle>e1, ns\<rangle> \<Down> LitV (LBool vc1)" and "A,\<Gamma>,\<Omega> \<turnstile> \<langle>e2, ns\<rangle> \<Down> LitV (LBool vc2)"
+  shows "A,\<Gamma>,\<Omega> \<turnstile> \<langle>e1 \<guillemotleft>Or\<guillemotright> e2, ns\<rangle> \<Down> LitV (LBool (vc1 \<or> vc2))"
   using assms
   by (auto intro: RedBinOp)
 
 lemma imp_vc_rel: 
-  assumes "A,\<Gamma> \<turnstile> \<langle>e1, ns\<rangle> \<Down> LitV (LBool vc1)" and "A,\<Gamma> \<turnstile> \<langle>e2, ns\<rangle> \<Down> LitV (LBool vc2)"
-  shows "A,\<Gamma> \<turnstile> \<langle>e1 \<guillemotleft>Imp\<guillemotright> e2, ns\<rangle> \<Down> LitV (LBool (vc1 \<longrightarrow> vc2))"
+  assumes "A,\<Gamma>,\<Omega> \<turnstile> \<langle>e1, ns\<rangle> \<Down> LitV (LBool vc1)" and "A,\<Gamma>,\<Omega> \<turnstile> \<langle>e2, ns\<rangle> \<Down> LitV (LBool vc2)"
+  shows "A,\<Gamma>,\<Omega> \<turnstile> \<langle>e1 \<guillemotleft>Imp\<guillemotright> e2, ns\<rangle> \<Down> LitV (LBool (vc1 \<longrightarrow> vc2))"
   using assms
   by (auto intro: RedBinOp)
 
 lemma not_vc_rel:
-  assumes "A,\<Gamma> \<turnstile> \<langle>e, ns\<rangle> \<Down> LitV (LBool vc)"
-  shows "A,\<Gamma> \<turnstile> \<langle>UnOp Not e, ns\<rangle> \<Down> LitV (LBool (\<not> vc))"
+  assumes "A,\<Gamma>,\<Omega> \<turnstile> \<langle>e, ns\<rangle> \<Down> LitV (LBool vc)"
+  shows "A,\<Gamma>,\<Omega> \<turnstile> \<langle>UnOp Not e, ns\<rangle> \<Down> LitV (LBool (\<not> vc))"
   using assms
   by (auto intro: RedUnOp)
 
 (* integer operations *)
 lemma add_vc_rel: 
-  assumes "A,\<Gamma> \<turnstile> \<langle>e1, ns\<rangle> \<Down> LitV (LInt vc1)" and "A,\<Gamma> \<turnstile> \<langle>e2, ns\<rangle> \<Down> LitV (LInt vc2)"
-  shows "A,\<Gamma> \<turnstile> \<langle>e1 \<guillemotleft>Add\<guillemotright> e2, ns\<rangle> \<Down> LitV (LInt (vc1 + vc2))"
+  assumes "A,\<Gamma>,\<Omega> \<turnstile> \<langle>e1, ns\<rangle> \<Down> LitV (LInt vc1)" and "A,\<Gamma>,\<Omega> \<turnstile> \<langle>e2, ns\<rangle> \<Down> LitV (LInt vc2)"
+  shows "A,\<Gamma>,\<Omega> \<turnstile> \<langle>e1 \<guillemotleft>Add\<guillemotright> e2, ns\<rangle> \<Down> LitV (LInt (vc1 + vc2))"
   using assms
   by (auto intro: RedBinOp)
 
 lemma sub_vc_rel: 
-  assumes "A,\<Gamma> \<turnstile> \<langle>e1, ns\<rangle> \<Down> LitV (LInt (vc1))" and "A,\<Gamma> \<turnstile> \<langle>e2, ns\<rangle> \<Down> LitV (LInt vc2)"
-  shows "A,\<Gamma> \<turnstile> \<langle>e1 \<guillemotleft>Sub\<guillemotright> e2, ns\<rangle> \<Down> LitV (LInt (vc1 - vc2))"
+  assumes "A,\<Gamma>,\<Omega> \<turnstile> \<langle>e1, ns\<rangle> \<Down> LitV (LInt (vc1))" and "A,\<Gamma>,\<Omega> \<turnstile> \<langle>e2, ns\<rangle> \<Down> LitV (LInt vc2)"
+  shows "A,\<Gamma>,\<Omega> \<turnstile> \<langle>e1 \<guillemotleft>Sub\<guillemotright> e2, ns\<rangle> \<Down> LitV (LInt (vc1 - vc2))"
   using assms
   by (auto intro: RedBinOp)
 
 lemma mul_vc_rel: 
-  assumes "A,\<Gamma> \<turnstile> \<langle>e1, ns\<rangle> \<Down> LitV (LInt vc1)" and "A,\<Gamma> \<turnstile> \<langle>e2, ns\<rangle> \<Down> LitV (LInt vc2)"
-  shows "A,\<Gamma> \<turnstile> \<langle>e1 \<guillemotleft>Mul\<guillemotright> e2, ns\<rangle> \<Down> LitV (LInt (vc1 * vc2))"
+  assumes "A,\<Gamma>,\<Omega> \<turnstile> \<langle>e1, ns\<rangle> \<Down> LitV (LInt vc1)" and "A,\<Gamma>,\<Omega> \<turnstile> \<langle>e2, ns\<rangle> \<Down> LitV (LInt vc2)"
+  shows "A,\<Gamma>,\<Omega> \<turnstile> \<langle>e1 \<guillemotleft>Mul\<guillemotright> e2, ns\<rangle> \<Down> LitV (LInt (vc1 * vc2))"
   using assms
   by (auto intro: RedBinOp)
 
 lemma uminus_vc_rel:
-  assumes "A,\<Gamma> \<turnstile> \<langle>e, ns\<rangle> \<Down> LitV (LInt vc)"
-  shows "A,\<Gamma> \<turnstile> \<langle>UnOp UMinus e, ns\<rangle> \<Down> LitV (LInt (- vc))"
+  assumes "A,\<Gamma>,\<Omega> \<turnstile> \<langle>e, ns\<rangle> \<Down> LitV (LInt vc)"
+  shows "A,\<Gamma>,\<Omega> \<turnstile> \<langle>UnOp UMinus e, ns\<rangle> \<Down> LitV (LInt (- vc))"
   using assms
   by (auto intro: RedUnOp)
 
 (* quantifiers *)
 lemma forall_vc_rel_general: 
-  assumes "\<And> i. A,\<Gamma> \<turnstile> \<langle>e, (env_shift ns)(0 \<mapsto> LitV (C i))\<rangle> \<Down> LitV (LBool (P i))" and
+  assumes "\<And> i. A,\<Gamma>,\<Omega> \<turnstile> \<langle>e, ext_env ns (LitV (C i))\<rangle> \<Down> LitV (LBool (P i))" and
           "\<And> i v. ty_val_rel A v (TPrim primty) \<Longrightarrow> \<exists>i. v = LitV (C i)"
           "\<And> i. ty_val_rel A (LitV (C i)) (TPrim primty)"
-  shows  "A,\<Gamma> \<turnstile> \<langle>Forall (TPrim primty) e, ns\<rangle> \<Down> LitV (LBool (\<forall>i. P i))"
+  shows  "A,\<Gamma>,\<Omega> \<turnstile> \<langle>Forall (TPrim primty) e, ns\<rangle> \<Down> LitV (LBool (\<forall>i. P i))"
 proof (cases "(\<forall>i. P i)")
   case True
   thus ?thesis using assms by (fastforce intro: RedForAllTrue)
 next
   case False
   from this obtain z where "\<not>(P z)" by auto
-  have "A,\<Gamma> \<turnstile> \<langle>Forall (TPrim primty) e, ns\<rangle> \<Down> LitV (LBool False)"
+  have "A,\<Gamma>,\<Omega> \<turnstile> \<langle>Forall (TPrim primty) e, ns\<rangle> \<Down> LitV (LBool False)"
     apply (rule RedForAllFalse[where ?v = "LitV (C z)"])
-    apply (simp only: assms)
+    apply simp
+    using assms(3) apply auto[1]
     by (metis (full_types) \<open>\<not> P z\<close> assms(1))
   then show ?thesis by (simp add: False)
 qed
 
 lemma exists_vc_rel_general:
-  assumes "\<And> i. A,\<Gamma> \<turnstile> \<langle>e, (env_shift ns)(0 \<mapsto> LitV (C i))\<rangle> \<Down> LitV (LBool (P i))"
+  assumes "\<And> i. A,\<Gamma>,\<Omega> \<turnstile> \<langle>e, ext_env ns (LitV (C i))\<rangle> \<Down> LitV (LBool (P i))"
           "\<And> i v. ty_val_rel A v (TPrim primty) \<Longrightarrow> \<exists>i. v = LitV (C i)"
           "\<And> i. ty_val_rel A (LitV (C i)) (TPrim primty)"
-  shows "A,\<Gamma> \<turnstile> \<langle>Exists (TPrim primty) e, ns\<rangle> \<Down> LitV (LBool (\<exists>i. P i))"
+  shows "A,\<Gamma>,\<Omega> \<turnstile> \<langle>Exists (TPrim primty) e, ns\<rangle> \<Down> LitV (LBool (\<exists>i. P i))"
 proof (cases "\<exists>i. P i")
   case True
   from this obtain z where "P z" by auto
-  have "A,\<Gamma> \<turnstile> \<langle>Exists (TPrim primty) e, ns\<rangle> \<Down> LitV (LBool True)"
+  have "A,\<Gamma>,\<Omega> \<turnstile> \<langle>Exists (TPrim primty) e, ns\<rangle> \<Down> LitV (LBool True)"
     apply (rule RedExistsTrue[where ?v = "LitV (C z)"])
-     apply (simp only: assms)
+    apply simp
+    using assms(3) apply auto[1]
     using assms \<open>P z\<close> by (metis (full_types))     
   thus ?thesis by (simp add: True)
 next
@@ -96,26 +98,26 @@ next
 qed
 
 lemma forall_vc_rel_int: 
-  assumes "\<And> i. A,\<Gamma> \<turnstile> \<langle>e, (env_shift ns)(0 \<mapsto> LitV (LInt i))\<rangle> \<Down> LitV (LBool (P i))"
-  shows  "A,\<Gamma> \<turnstile> \<langle>Forall (TPrim TInt) e, ns\<rangle> \<Down> LitV (LBool (\<forall>i. P i))"
+  assumes "\<And> i. A,\<Gamma>,\<Omega> \<turnstile> \<langle>e, ext_env ns (LitV (LInt i))\<rangle> \<Down> LitV (LBool (P i))"
+  shows  "A,\<Gamma>,\<Omega> \<turnstile> \<langle>Forall (TPrim TInt) e, ns\<rangle> \<Down> LitV (LBool (\<forall>i. P i))"
   using assms
   by (rule forall_vc_rel_general, auto elim: type_of_val_int_elim)
 
 lemma forall_vc_rel_bool: 
-  assumes "\<And> b. A,\<Gamma> \<turnstile> \<langle>e, (env_shift ns)(0 \<mapsto> LitV (LBool b))\<rangle> \<Down> LitV (LBool (P b))"
-  shows  "A,\<Gamma> \<turnstile> \<langle>Forall (TPrim TBool) e, ns\<rangle> \<Down> LitV (LBool (\<forall>b. P b))"
+  assumes "\<And> b. A,\<Gamma>,\<Omega> \<turnstile> \<langle>e, ext_env ns (LitV (LBool b))\<rangle> \<Down> LitV (LBool (P b))"
+  shows  "A,\<Gamma>,\<Omega> \<turnstile> \<langle>Forall (TPrim TBool) e, ns\<rangle> \<Down> LitV (LBool (\<forall>b. P b))"
   using assms
   by (rule forall_vc_rel_general, auto elim: type_of_val_bool_elim)
 
 lemma exists_vc_rel_int:
-  assumes "\<And> i. A,\<Gamma> \<turnstile> \<langle>e, (env_shift ns)(0 \<mapsto> LitV (LInt i))\<rangle> \<Down> LitV (LBool (P i))"
-  shows "A,\<Gamma> \<turnstile> \<langle>Exists (TPrim TInt) e, ns\<rangle> \<Down> LitV (LBool (\<exists>i. P i))"
+  assumes "\<And> i. A,\<Gamma>,\<Omega> \<turnstile> \<langle>e, ext_env ns (LitV (LInt i))\<rangle> \<Down> LitV (LBool (P i))"
+  shows "A,\<Gamma>,\<Omega> \<turnstile> \<langle>Exists (TPrim TInt) e, ns\<rangle> \<Down> LitV (LBool (\<exists>i. P i))"
   using assms
   by (rule exists_vc_rel_general, auto elim: type_of_val_int_elim)
 
 lemma exists_vc_rel_bool:
-  assumes "\<And> b. A,\<Gamma> \<turnstile> \<langle>e, (env_shift ns)(0 \<mapsto> LitV (LBool b))\<rangle> \<Down> LitV (LBool (P b))"
-  shows "A,\<Gamma> \<turnstile> \<langle>Exists (TPrim TBool) e, ns\<rangle> \<Down> LitV (LBool (\<exists>b. P b))"
+  assumes "\<And> b. A,\<Gamma>,\<Omega> \<turnstile> \<langle>e, ext_env ns (LitV (LBool b))\<rangle> \<Down> LitV (LBool (P b))"
+  shows "A,\<Gamma>,\<Omega> \<turnstile> \<langle>Exists (TPrim TBool) e, ns\<rangle> \<Down> LitV (LBool (\<exists>b. P b))"
   using assms
   by (rule exists_vc_rel_general, auto elim: type_of_val_bool_elim)
 
